app/Encode.v
@@ -1,0 +1,63 @@
+From JSON Require Export
+     Operator.
+From AsyncTest Require Export
+     Classes
+     Operator.
+From App Require Export
+     AppMessage.
+Import
+  XNotations.
+Open Scope jexp_scope.
+
+Instance XEncode__Request : XEncode (swap_request id) :=
+  fun r =>
+    jobj "method" (swap_path r) +
+    match r with
+    | Request__ListAccount uid =>
+      jobj "user" uid
+    | Request__TakeOrder uid oid =>
+      jobj "user" uid + jobj "order" oid
+    | Request__MakeOrder uid bt ba st sa =>
+      jobj "user" uid + jobj "buyTicker" bt + jobj "buyAmount" ba +
+      jobj "sellTicker" st + jobj "sellAmount" sa
+    | Request__Deposit  uid t a
+    | Request__Withdraw uid t a =>
+      jobj "user" uid + jobj "ticker" t + jobj "amount" a
+    | Request__Clean
+    | Request__ListOrders => Jexp__Object []
+    end.
+
+Close Scope jexp_scope.
+
+Import
+  Encode
+  JNotations.
+Open Scope json_scope.
+
+Instance JEncode__Account : JEncode (accountT id) :=
+  fun a => let '(aid, (uid, tkr, amt)) := a in
+         jobj "ID"          aid +
+         jobj "UserID"      uid +
+         jobj "AssetTicker" tkr +
+         jobj "Amount"      amt.
+
+Instance JEncode__Order : JEncode (orderT id) :=
+  fun o => let '(oid, (bid, bam, sid, sam)) := o in
+         jobj "ID"         oid +
+         jobj "BuyerID"    bid +
+         jobj "BuyAmount"  bam +
+         jobj "SellerID"   sid +
+         jobj "SellAmount" sam.
+
+Instance JEncode__Response : JEncode (swap_response id) :=
+  fun r =>
+    jobj "code" (swap_code r) +
+    match r with
+    | Response__ListAccount l => jobj "accounts" l
+    | Response__ListOrders  l => jobj "orders"   l
+    | Response__Account x
+    | Response__Order   x     => encode x
+    | _ => JSON__Object []
+    end.
+
+Close Scope json_scope.
